msl_ext/alg_seplog.v
@@ -1,0 +1,2 @@
+Require Import VST.msl.alg_seplog.
+Require Import RamifyCoq.msl_ext.seplog.
